DenotSem/Types.thy
@@ -1,0 +1,5 @@
+theory Types
+ imports Values
+begin
+
+end
